pcuic/theories/PCUICRelevance.v
@@ -4,51 +4,6 @@ From MetaCoq.PCUIC Require Import PCUICAst PCUICAstUtils.
 
 Require Import ssreflect.
 
-Definition mark_context := list relevance.
-Definition marks_of_context (Γ: context) := List.map (binder_relevance ∘ decl_name) Γ.
-
-Inductive isTermRel (Σ : global_env) (Γ : mark_context) : term -> relevance -> Type :=
-  | rel_Rel n rel :
-      nth_error Γ n = Some rel -> isTermRel Σ Γ (tRel n) rel
-
-  | rel_Lambda na A t rel :
-      isTermRel Σ (Γ ,, na.(binder_relevance)) t rel -> isTermRel Σ Γ (tLambda na A t) rel
-  
-  | rel_LetIn na b B t rel :
-      isTermRel Σ (Γ ,, na.(binder_relevance)) t rel -> isTermRel Σ Γ (tLetIn na b B t) rel
-  
-  | rel_App t u rel :
-      isTermRel Σ Γ t rel -> isTermRel Σ Γ (tApp t u) rel
-  
-  | rel_Const kn u decl :
-      declared_constant Σ kn decl -> isTermRel Σ Γ (tConst kn u) decl.(cst_relevance)
-  
-  | rel_Construct ind i u mdecl idecl cdecl :
-      declared_constructor Σ (ind, i) mdecl idecl cdecl -> isTermRel Σ Γ (tConstruct ind i u) idecl.(ind_relevance)
-  
-  | rel_Case ci p c brs :
-      isTermRel Σ Γ (tCase ci p c brs) ci.(ci_relevance)
-  
-  | rel_Proj p u mdecl idecl cdecl pdecl :
-      declared_projection Σ p mdecl idecl cdecl pdecl -> isTermRel Σ Γ (tProj p u) pdecl.(proj_relevance)
-  
-  | rel_Fix mfix n def :
-      nth_error mfix n = Some def -> isTermRel Σ Γ (tFix mfix n) def.(dname).(binder_relevance)
-  
-  | rel_CoFix mfix n def :
-      nth_error mfix n = Some def -> isTermRel Σ Γ (tCoFix mfix n) def.(dname).(binder_relevance)
-  
-  | rel_Sort s :
-      isTermRel Σ Γ (tSort s) Relevant
-  
-  | rel_Prod na A B :
-      isTermRel Σ Γ (tProd na A B) Relevant
-  
-  | rel_Ind ind u :
-      isTermRel Σ Γ (tInd ind u) Relevant. 
-
-Derive Signature for isTermRel.
-
 Lemma mark_of_context_app Γ Γ' Δ Δ' :
   marks_of_context Γ = marks_of_context Γ' -> marks_of_context Δ = marks_of_context Δ' -> marks_of_context (Γ,,, Δ) = marks_of_context (Γ',,, Δ').
 Proof.
