pcuic/theories/Conversion/PCUICWeakeningEnvConv.v
@@ -49,7 +49,7 @@ Qed.
 Section ExtendsWf.
   Context {cf : checker_flags}.
   Context {Pcmp: global_env_ext -> context -> conv_pb -> term -> term -> Type}.
-  Context {P: global_env_ext -> context -> term -> typ_or_sort -> Type}.
+  Context {P: global_env_ext -> context -> judgment -> Type}.
 
   Let wf := on_global_env Pcmp P.
 
